src/program_proof/memkv/memkv_clerk_proof.v
@@ -2,383 +2,346 @@ From Perennial.program_proof Require Import grove_prelude std_proof.
 From Goose.github_com.mit_pdos.gokv Require Import memkv.
 From Perennial.program_proof.lockservice Require Import rpc.
 From Perennial.program_logic Require Import atomic_fupd.
-From Perennial.program_proof.memkv Require Export common_proof memkv_coord_definitions memkv_coord_clerk_proof memkv_shard_clerk_proof.
+From Perennial.program_proof.memkv Require Export common_proof memkv_coord_definitions memkv_seq_clerk_proof.
 
-Section memkv_clerk_proof.
+Section memkv_concurrent_clerk_proof.
 
 Context `{!heapGS Σ (ext:=grove_op) (ffi:=grove_model), !rpcG Σ ShardReplyC, !rpcregG Σ, !kvMapG Σ}.
 
-Definition own_MemKVClerk (ck:loc) (γ:gname) : iProp Σ :=
-  ∃ (s coordCk:loc) shardMap_sl (shardMapping:list u64),
-  "HshardClerks" ∷ ck ↦[MemKVClerk :: "shardClerks"] #s ∗
-  "HshardClerksSet" ∷ own_ShardClerkSet s γ ∗
-  "HcoordCk" ∷ ck ↦[MemKVClerk :: "coordCk"] #coordCk ∗
-  "HcoordCk_own" ∷ own_MemKVCoordClerk coordCk γ ∗
-  "HshardMap" ∷ ck ↦[MemKVClerk :: "shardMap"] (slice_val shardMap_sl) ∗
-  "HshardMap_sl" ∷ is_slice shardMap_sl uint64T 1%Qp shardMapping ∗
-  "%HshardMap_length" ∷ ⌜Z.of_nat (length shardMapping) = uNSHARD⌝ ∗
-  "#HshardServers" ∷ all_are_shard_servers shardMapping γ
+Local Definition own_KVClerk (p:loc) (γ:gname) : iProp Σ :=
+  ∃ (freeClerks_sl:Slice.t) (freeClerks:list loc),
+  "HfreeClerks" ∷ p ↦[KVClerk :: "freeClerks"] (slice_val freeClerks_sl) ∗
+  "HfreeClerks_sl" ∷ is_slice (V:=loc) freeClerks_sl seqKVClerkPtr 1 freeClerks ∗
+  "HfreeClerks_own" ∷ [∗ list] ck ∈ freeClerks, own_SeqKVClerk ck γ
 .
 
-Lemma wp_MakeMemKVClerk (coord:u64) cm γ :
-  {{{
-       is_coord_server coord γ ∗ is_ConnMan cm
-  }}}
-    MakeMemKVClerk #coord #cm
-  {{{
-       (ck:loc), RET #ck; own_MemKVClerk ck γ.(coord_kv_gn)
-  }}}
+(* FIXME: imports are screwed somewhere, [val] is shadowed the wrong way. *)
+Definition is_KVClerk (p_ptr:loc) (γ:gname) : iProp Σ :=
+  ∃ (coord:u64) mu (cm:loc) (γcoord:server_chan_gnames),
+  "#Hmu" ∷ readonly (p_ptr ↦[KVClerk :: "mu"] mu) ∗
+  "#Hcoord" ∷ readonly (p_ptr ↦[KVClerk :: "coord"] #coord) ∗
+  "#Hcm" ∷ readonly (p_ptr ↦[KVClerk :: "cm"] #cm) ∗
+  "#Hiscoord" ∷ is_coord_server coord (Build_memkv_coord_names γcoord γ) ∗
+  "#Hinv" ∷ is_lock nroot mu (own_KVClerk p_ptr γ) ∗
+  "#Hiscm" ∷ is_ConnMan cm
 .
+
+Local Lemma wp_KVClerk__getSeqClerk p γ :
+  is_KVClerk p γ -∗
+  {{{ True }}}
+    KVClerk__getSeqClerk #p
+  {{{ (ck:loc), RET #ck; own_SeqKVClerk ck γ }}}.
 Proof.
-  iIntros (Φ) "[#Hcoord #Hcm] HΦ".
-  rewrite /MakeMemKVClerk.
+  iIntros "#Hcck !> %Φ _ HΦ".
   wp_lam.
-  wp_apply (wp_allocStruct).
-  { Transparent slice.T. repeat econstructor.  Opaque slice.T. }
-  iIntros (cck) "Hcck".
+  iNamed "Hcck".
+  wp_loadField.
+  wp_apply (acquire_spec with "Hinv").
+  iIntros "[Hlocked Hown]". iNamed "Hown".
   wp_pures.
-  wp_apply (wp_allocStruct).
-  { Transparent slice.T. repeat econstructor.  Opaque slice.T. }
-  iIntros (ck) "Hck".
-  iDestruct (struct_fields_split with "Hck") as "HH".
-  iNamed "HH".
-  iDestruct (struct_fields_split with "Hcck") as "HH".
-  iNamed "HH".
+  wp_loadField.
+  wp_apply wp_slice_len.
   wp_pures.
-  wp_storeField.
-  wp_loadField.
-  wp_storeField.
-  wp_loadField.
-  wp_storeField.
-  wp_bind (MakeShardClerkSet _).
-  wp_lam.
-  replace (ref (InjLV #null))%E with (NewMap (struct.ptrT MemKVShardClerk)) by auto.
-  wp_apply (wp_NewMap).
-  iIntros (mref_set) "Hmap_set".
-  wp_apply (wp_allocStruct).
-  { eauto. }
-  iIntros (clset) "Hset".
-  wp_storeField.
-  wp_loadField.
-  wp_apply (wp_MemKVCoordClerk__GetShardMap with "[c host]").
-  { rewrite /own_MemKVCoordClerk. iExists _, _, _. iFrame "c host Hcm".
-    iSplit; last first.
-    { iExact "Hcoord". }
-    done.
-  }
-  iIntros (shardMap_sl shardMapping) "(Hcck & HshardMap_sl & %Hlen & #Hall_are_shard_servers)".
-  Transparent slice.T.
-  wp_storeField.
-  Opaque slice.T.
-  iModIntro. iApply "HΦ".
-  iExists _, _, _, _. iFrame.
-  iFrame "% #". iExists _, _, _.
-  iFrame "Hmap_set Hcm".
-  iDestruct (struct_fields_split with "Hset") as "HH".
-  iNamed "HH". iFrame.
-  rewrite big_sepM_empty; done.
+  destruct (decide (int.nat freeClerks_sl.(Slice.sz) = 0)) as [Hzero|Hnzero].
+  - (* creating new clerk *)
+    rewrite bool_decide_true; last first.
+    { do 2 f_equal. word. }
+    wp_loadField.
+    wp_apply (release_spec'' with "Hinv [-HΦ]").
+    { iFrame. rewrite /own_KVClerk. eauto with iFrame. }
+    wp_pures.
+    wp_loadField.
+    wp_loadField.
+    wp_apply (wp_MakeSeqKVClerk with "[$Hiscoord $Hiscm]").
+    iIntros (ck) "Hck".
+    iApply "HΦ".
+    eauto.
+  - (* using existing clerk *)
+    rewrite bool_decide_false; last first.
+    { intros [=Hz]. apply Hnzero. rewrite Hz. word. }
+    wp_loadField.
+    iDestruct (is_slice_sz with "HfreeClerks_sl") as %Hlen.
+    destruct freeClerks as [|freeClerks Hck _] using rev_ind.
+    { exfalso. apply Hnzero. done. }
+    rewrite app_length in Hlen. simpl in Hlen.
+    rewrite big_sepL_snoc.
+    iDestruct (is_slice_small_read with "HfreeClerks_sl") as "[HfreeClerks_sl HfreeClerks_close]".
+    wp_apply (wp_SliceGet (V:=loc) with "[$HfreeClerks_sl]").
+    { iPureIntro.
+      replace (int.nat (word.sub freeClerks_sl.(Slice.sz) 1%Z)) with (int.nat freeClerks_sl.(Slice.sz) - 1) by word.
+      rewrite lookup_app_r; last by word. rewrite -Hlen.
+      replace (length Hck + 1 - 1 - length Hck) with 0 by lia.
+      done. }
+    iIntros "HfreeClerks_sl".
+
+    wp_loadField.
+    wp_apply wp_SliceTake.
+    { word. }
+    wp_bind (struct.storeF _ _ _ _).
+    (* FIXME why do we have to apply storeField by hand here? *)
+    iApply (wp_storeField with "HfreeClerks").
+    { rewrite /field_ty. simpl. val_ty. }
+    iIntros "!> HfreeClerks".
+    iDestruct "HfreeClerks_own" as "[HfreeClerks_own Hck]".
+    wp_loadField.
+    iDestruct ("HfreeClerks_close" with "HfreeClerks_sl") as "HfreeClerks_sl".
+    wp_apply (release_spec'' with "Hinv [$Hlocked HfreeClerks_own HfreeClerks_sl HfreeClerks]").
+    { rewrite /own_KVClerk. iModIntro. iExists _, _. iFrame.
+      (* FIXME need typed slice lemma *)
+      iClear "#".
+      rewrite /is_slice.
+      iDestruct (is_slice_take_cap _ _ _ (length Hck) with "HfreeClerks_sl") as "HfreeClerks_sl".
+      { rewrite /list.untype fmap_length app_length /=. word. }
+      rewrite /list.untype fmap_app take_app_alt; last first.
+      { rewrite fmap_length. word. }
+      replace (word.sub freeClerks_sl.(Slice.sz) 1%Z) with (length Hck : u64) by word.
+      iFrame. }
+    wp_pures. iApply "HΦ".
+    eauto.
 Qed.
 
-Lemma wp_MemKVClerk__Get (ck:loc) (γ:gname) (key:u64) :
-⊢ {{{ own_MemKVClerk ck γ }}}
+Local Lemma wp_KVClerk__putSeqClerk p γ ck :
+  is_KVClerk p γ -∗
+  {{{ own_SeqKVClerk ck γ }}}
+    KVClerk__putSeqClerk #p #ck
+  {{{ RET #(); True }}}.
+Proof.
+  iIntros "#Hcck !> %Φ Hck HΦ". wp_lam.
+  wp_apply (wp_fork with "[Hck]").
+  { iModIntro.
+    iNamed "Hcck".
+    wp_loadField.
+    wp_apply (acquire_spec with "Hinv").
+    iIntros "[Hlocked Hown]". iNamed "Hown".
+    wp_loadField.
+    wp_apply (wp_SliceAppend with "HfreeClerks_sl").
+    iIntros (freeClerks_sl') "HfreeClerks_sl".
+    wp_bind (struct.storeF _ _ _ _).
+    (* FIXME why do we have to apply storeField by hand here? *)
+    iApply (wp_storeField with "HfreeClerks").
+    { rewrite /field_ty. simpl. val_ty. }
+    iIntros "!> HfreeClerks".
+    wp_loadField.
+    wp_apply (release_spec'' with "Hinv [$Hlocked HfreeClerks_own HfreeClerks_sl HfreeClerks Hck]").
+    { rewrite /own_KVClerk. iModIntro. iExists _, _. iFrame.
+      rewrite big_sepL_singleton. done. }
+    done.
+  }
+  by iApply "HΦ".
+Qed.
+
+Lemma wp_MakeKVClerk coord cm γ :
+  is_coord_server coord γ -∗
+  is_ConnMan cm -∗
+  {{{ True }}}
+    MakeKVClerk #coord #cm
+  {{{ (p:loc), RET #p; is_KVClerk p γ.(coord_kv_gn) }}}.
+Proof.
+  iIntros "#Hcoord #Hcm !> %Φ _ HΦ". wp_lam.
+  wp_apply (wp_allocStruct).
+  { Transparent slice.T. val_ty. Opaque slice.T. }
+  iIntros (l) "Hl".
+  iDestruct (struct_fields_split with "Hl") as "HH". iNamed "HH".
+  wp_apply wp_new_free_lock.
+  iIntros (mu) "Hfreelock".
+  wp_storeField.
+  wp_storeField.
+  wp_storeField.
+  wp_apply (wp_NewSlice (V:=loc)).
+  iIntros (freeClerks_sl) "HfreeClerks_sl".
+  (* FIXME why do we have to apply storeField by hand here? *)
+  wp_apply (wp_storeField with "freeClerks").
+  { rewrite /field_ty. simpl. val_ty. }
+  iIntros "HfreeClerks".
+  iMod (alloc_lock with "Hfreelock [HfreeClerks HfreeClerks_sl]") as "Hlock"; last first.
+  { wp_pures. iApply "HΦ". rewrite /is_KVClerk.
+    iExists coord, #mu, _, γ.(coord_urpc_gn). iFrame "Hcoord Hlock".
+    iMod (readonly_alloc_1 with "mu") as "$".
+    iMod (readonly_alloc_1 with "coord") as "$".
+    iMod (readonly_alloc_1 with "cm") as "$".
+    eauto with iFrame. }
+  rewrite /own_KVClerk. iExists _, _. iFrame.
+  rewrite big_sepL_nil. done.
+Qed.
+
+Lemma wp_KVClerk__Get (p:loc) (γ:gname) (key:u64) :
+⊢ {{{ is_KVClerk p γ }}}
   <<< ∀∀ v, kvptsto γ key v >>>
-    MemKVClerk__Get #ck #key @ ∅
+    KVClerk__Get #p #key @ ∅
   <<< kvptsto γ key v >>>
   {{{ val_sl q, RET slice_val val_sl;
-      own_MemKVClerk ck γ ∗ is_slice_small val_sl byteT q%Qp v
+      is_slice_small val_sl byteT q%Qp v
   }}}.
-Proof using Type*.
-  iIntros "!#" (Φ) "Hown Hatomic".
-  wp_lam.
-  wp_pures.
-  wp_apply wp_ref_of_zero.
-  { done. }
-  iIntros (rep_ptr) "Hrep".
-  wp_pures.
-
-  (* Weaken assumption for loop invariant *)
-  iAssert (∃ rep_sl, rep_ptr ↦[slice.T byteT] (slice_val rep_sl) )%I with "[Hrep]" as "Hrep".
-  {
-    rewrite zero_slice_val.
-    iExists _; iFrame.
-  }
-
-  wp_forBreak.
-  wp_pures.
-
-  wp_apply (wp_shardOf_bound).
-  iIntros (sid HsidLe).
-  wp_pures.
-
-  iNamed "Hown".
-  wp_loadField.
-  iDestruct (is_slice_small_acc with "HshardMap_sl") as "[Hsmall_sl HslClose]".
-
-  assert (int.nat sid < length shardMapping)%nat as HsidLe_nat by word.
-  eapply list_lookup_lt in HsidLe_nat.
-  destruct HsidLe_nat as [hostID HsidLe_nat].
-  wp_apply (wp_SliceGet (V:=u64) with "[$Hsmall_sl]").
-  {
-    iPureIntro.
-    done.
-  }
-  iIntros "Hsmall_sl".
-  wp_pures.
-  wp_loadField.
-
-  unfold all_are_shard_servers.
-  iDestruct ("HshardServers" $! (int.nat sid) hostID HsidLe_nat) as "HH".
-  iNamed "HH".
-
-  wp_apply (wp_ShardClerkSet__GetClerk with "[$HshardClerksSet]").
-  { iFrame "HH". }
-  iClear "HH".
-
-  iIntros (?) "(HshardCk & HcloseShardSet)".
-
-  wp_pures.
-  rewrite difference_empty_L.
-  wp_apply (wp_MemKVShardClerk__Get with "[Hatomic $HshardCk $Hrep]").
-  {
-    iFrame "Hatomic".
-  }
-  iIntros (e) "HshardGetPost".
-  wp_pures.
-  wp_if_destruct.
-  {
-    iRight.
-    iModIntro.
-    iSplitL ""; first done.
-    wp_pures.
-    iDestruct "HshardGetPost" as "(HshardCk & [[%Hbad _]|[_ Hpost]])".
-    { by exfalso. }
-    iNamed "Hpost".
-    iDestruct "Hpost" as "(Hrep & Hval_sl & HΦ)".
-    wp_load.
-    iMod (readonly_load with "Hval_sl") as (?) "Hval_sl".
-    iModIntro.
-    iApply "HΦ".
-    iFrame.
-    iDestruct ("HcloseShardSet" with "HshardCk") as "HshardSet".
-    iDestruct ("HslClose" with "Hsmall_sl") as "?".
-    iExists _, _, _, _. by iFrame "#∗".
-  }
-  {
-    wp_loadField.
-    iDestruct "HshardGetPost" as "(HshardCk & [Hatomic|[%Hbad _]])"; last first.
-    { exfalso. naive_solver. }
-    iDestruct ("HcloseShardSet" with "HshardCk") as "HshardSet".
-    wp_apply (wp_MemKVCoordClerk__GetShardMap with "[$HcoordCk_own]").
-    iIntros (shardMap_sl' shardMapping') "(HcoordCk_own & HshardMap_sl & %Hlength & #HshardServers')".
-    wp_apply (wp_storeField with "HshardMap").
-    { apply slice_val_ty. }
-    iIntros "HshardMap".
-    wp_pures.
-    iLeft.
-    iModIntro.
-
-    iSplitL ""; first done.
-    iDestruct "Hatomic" as "[_ $]".
-    iExists _,_,_,_; by iFrame "#∗".
-  }
+Proof.
+  iIntros "!#" (Φ) "#Hp Hatomic". wp_lam.
+  wp_apply (wp_KVClerk__getSeqClerk with "Hp").
+  iIntros (ck) "Hck".
+  wp_apply (wp_SeqKVClerk__Get with "Hck").
+  iMod "Hatomic" as (v) "[Hkv HΦ]".
+  iModIntro. iExists v. iFrame "Hkv".
+  iIntros "Hkv". iMod ("HΦ" with "Hkv") as "HΦ".
+  iIntros "!> %val_sl %q [Hck Hsl]".
+  wp_apply (wp_KVClerk__putSeqClerk with "Hp Hck").
+  wp_pures. iApply "HΦ". done.
 Qed.
 
-(* Sequential spec *)
-Lemma wp_MemKVClerk__Get_seq (ck:loc) (γ:gname) (key:u64) (v:list u8) :
-  {{{ own_MemKVClerk ck γ ∗ kvptsto γ key v }}}
-    MemKVClerk__Get #ck #key @ ⊤
+(* Sequential spec (for when you have full ownership of the [kvptsto]) *)
+Lemma wp_KVClerk__Get_seq (p:loc) (γ:gname) (key:u64) (v:list u8) :
+  {{{ is_KVClerk p γ ∗ kvptsto γ key v }}}
+    KVClerk__Get #p #key @ ⊤
   {{{ val_sl q, RET slice_val val_sl;
-      own_MemKVClerk ck γ ∗ kvptsto γ key v ∗ is_slice_small val_sl byteT q%Qp v
+      kvptsto γ key v ∗ is_slice_small val_sl byteT q%Qp v
   }}}.
-Proof using Type*.
+Proof.
   iIntros (Φ) "(Hclerk & Hkey) HΦ".
-  iApply (wp_MemKVClerk__Get with "Hclerk").
+  iApply (wp_KVClerk__Get with "Hclerk").
   iApply fupd_mask_intro; first done. iNext.
   iIntros "Hclose". iExists _. iFrame "Hkey".
   iIntros "Hkey". iMod "Hclose" as "_". iModIntro.
   iIntros (??) "[Hclerk Hsl]". iApply "HΦ". iFrame.
 Qed.
 
-Lemma wp_MemKVClerk__Put (ck:loc) (γ:gname) (key:u64) (val_sl:Slice.t) (v:list u8):
-⊢ {{{ own_MemKVClerk ck γ ∗ readonly (is_slice_small val_sl byteT 1 v) }}}
+Lemma wp_KVClerk__Put (p:loc) (γ:gname) (key:u64) (val_sl:Slice.t) (v:list u8) :
+⊢ {{{ is_KVClerk p γ ∗ readonly (is_slice_small val_sl byteT 1 v) }}}
   <<< ∀∀ oldv, kvptsto γ key oldv >>>
-    MemKVClerk__Put #ck #key (slice_val val_sl) @ ∅
+    KVClerk__Put #p #key (slice_val val_sl) @ ∅
   <<< kvptsto γ key v >>>
-  {{{ RET #(); own_MemKVClerk ck γ }}}.
-Proof using Type*.
-  iIntros "!#" (Φ) "[Hown #Hval_sl] Hatomic".
-  wp_lam.
-  wp_pures.
-
-  wp_forBreak.
-  wp_pures.
-
-  wp_apply (wp_shardOf_bound).
-  iIntros (sid HsidLe).
-  wp_pures.
-
-  iNamed "Hown".
-  wp_loadField.
-  iDestruct (is_slice_small_acc with "HshardMap_sl") as "[Hsmall_sl HslClose]".
-
-  assert (int.nat sid < length shardMapping)%nat as HsidLe_nat by word.
-  eapply list_lookup_lt in HsidLe_nat.
-  destruct HsidLe_nat as [hostID HsidLe_nat].
-  wp_apply (wp_SliceGet (V:=u64) with "[$Hsmall_sl]").
-  {
-    iPureIntro.
-    done.
-  }
-  iIntros "Hsmall_sl".
-  wp_pures.
-  wp_loadField.
-
-  unfold all_are_shard_servers.
-  iDestruct ("HshardServers" $! (int.nat sid) hostID HsidLe_nat) as "HH".
-  iNamed "HH".
-  wp_apply (wp_ShardClerkSet__GetClerk with "[$HshardClerksSet $HH]").
-  iClear "HH".
-
-  iIntros (?) "(HshardCk & HcloseShardSet)".
-
-  wp_pures.
-  rewrite difference_empty_L.
-  wp_apply (wp_MemKVShardClerk__Put with "[Hatomic $Hval_sl $HshardCk]").
-  {
-    iFrame "Hatomic".
-  }
-  iIntros (e) "HshardPutPost".
-  wp_pures.
-  wp_if_destruct.
-  {
-    iRight.
-    iModIntro.
-    iSplitL ""; first done.
-    wp_pures.
-    iDestruct "HshardPutPost" as "(HshardCk & [[%Hbad _]|[_ Hpost]])".
-    { by exfalso. }
-    iApply "Hpost".
-    iDestruct ("HcloseShardSet" with "HshardCk") as "HshardSet".
-    iDestruct ("HslClose" with "Hsmall_sl") as "?".
-    iModIntro. iExists _, _, _, _. by iFrame "#∗".
-  }
-  {
-    wp_loadField.
-    iDestruct "HshardPutPost" as "(HshardCk & [Hatomic|[%Hbad _]])"; last first.
-    { exfalso. naive_solver. }
-    iDestruct ("HcloseShardSet" with "HshardCk") as "HshardSet".
-    wp_apply (wp_MemKVCoordClerk__GetShardMap with "[$HcoordCk_own]").
-    iIntros (shardMap_sl' shardMapping') "(HcoordCk_own & HshardMap_sl & %Hlength & #HshardServers')".
-    wp_apply (wp_storeField with "HshardMap").
-    { apply slice_val_ty. }
-    iIntros "HshardMap".
-    wp_pures.
-    iLeft.
-    iModIntro.
-
-    iSplitL ""; first done.
-    iDestruct "Hatomic" as "[_ $]".
-    iFrame.
-    iExists _,_,_,_. by iFrame "#∗".
-  }
+  {{{ RET #(); True }}}.
+Proof.
+  iIntros "!#" (Φ) "#[Hp Hsl] Hatomic". wp_lam.
+  wp_apply (wp_KVClerk__getSeqClerk with "Hp").
+  iIntros (ck) "Hck".
+  wp_apply (wp_SeqKVClerk__Put with "[$Hck $Hsl]").
+  iMod "Hatomic" as (oldv) "[Hkv HΦ]".
+  iModIntro. iExists oldv. iFrame "Hkv".
+  iIntros "Hkv". iMod ("HΦ" with "Hkv") as "HΦ".
+  iIntros "!> Hck".
+  wp_apply (wp_KVClerk__putSeqClerk with "Hp Hck").
+  iApply "HΦ". done.
 Qed.
 
-Lemma wp_MemKVClerk__ConditionalPut (ck:loc) (γ:gname) (key:u64) (expv_sl newv_sl:Slice.t) (expv newv:list u8):
-⊢ {{{ own_MemKVClerk ck γ ∗
+Lemma wp_KVClerk__Put_seq (p:loc) (γ:gname) (key:u64) (val_sl:Slice.t) (v oldv:list u8) :
+  {{{ is_KVClerk p γ ∗ readonly (is_slice_small val_sl byteT 1 v) ∗ kvptsto γ key oldv }}}
+    KVClerk__Put #p #key (slice_val val_sl) @ ⊤
+  {{{ RET #(); kvptsto γ key v }}}.
+Proof.
+  iIntros (Φ) "(Hclerk & Hsl & Hkey) HΦ".
+  iApply (wp_KVClerk__Put with "[$Hclerk $Hsl]").
+  iApply fupd_mask_intro; first done. iNext.
+  iIntros "Hclose". iExists _. iFrame "Hkey".
+  iIntros "Hkey". iMod "Hclose" as "_". iModIntro.
+  iIntros "_". iApply "HΦ". iFrame.
+Qed.
+
+Lemma wp_KVClerk__ConditionalPut (p:loc) (γ:gname) (key:u64) (expv_sl newv_sl:Slice.t) (expv newv:list u8):
+⊢ {{{ is_KVClerk p γ ∗
       readonly (is_slice_small expv_sl byteT 1 expv) ∗
       readonly (is_slice_small newv_sl byteT 1 newv) }}}
   <<< ∀∀ oldv, kvptsto γ key oldv >>>
-    MemKVClerk__ConditionalPut #ck #key (slice_val expv_sl) (slice_val newv_sl) @ ∅
+    KVClerk__ConditionalPut #p #key (slice_val expv_sl) (slice_val newv_sl) @ ∅
   <<< kvptsto γ key (if bool_decide (expv = oldv) then newv else oldv) >>>
-  {{{ RET #(bool_decide (expv = oldv));
-      own_MemKVClerk ck γ }}}.
-Proof using Type*.
-  iIntros "!#" (Φ) "(Hown & #Hexpv_sl & #Hnewv_sl) Hatomic".
-  wp_lam.
-  wp_pures.
-  wp_apply (wp_ref_of_zero _ _ boolT).
-  { done. }
-  iIntros (succ_ptr) "Hsucc".
-  wp_pures.
-  (* Weaken assumption for loop invariant *)
-  iAssert (∃ b:bool, succ_ptr ↦[boolT] #b)%I with "[Hsucc]" as "Hsucc".
-  { iExists _. done. }
-
-  wp_forBreak.
-  wp_pures.
-
-  wp_apply (wp_shardOf_bound).
-  iIntros (sid HsidLe).
-  wp_pures.
-
-  iNamed "Hown".
-  wp_loadField.
-  iDestruct (is_slice_small_acc with "HshardMap_sl") as "[Hsmall_sl HslClose]".
-
-  assert (int.nat sid < length shardMapping)%nat as HsidLe_nat by word.
-  eapply list_lookup_lt in HsidLe_nat.
-  destruct HsidLe_nat as [hostID HsidLe_nat].
-  wp_apply (wp_SliceGet (V:=u64) with "[$Hsmall_sl]").
-  {
-    iPureIntro.
-    done.
-  }
-  iIntros "Hsmall_sl".
-  wp_pures.
-  wp_loadField.
-
-  unfold all_are_shard_servers.
-  iDestruct ("HshardServers" $! (int.nat sid) hostID HsidLe_nat) as "HH".
-  iNamed "HH".
-  wp_apply (wp_ShardClerkSet__GetClerk with "[$HshardClerksSet $HH]").
-  iClear "HH".
-
-  iIntros (?) "(HshardCk & HcloseShardSet)".
-
-  wp_pures.
-  rewrite difference_empty_L.
-  wp_apply (wp_MemKVShardClerk__ConditionalPut _ _ _ _ _ _ _ _ (λ b, own_MemKVClerk ck γ -∗ Φ #b)%I
-    with "[Hatomic $HshardCk Hsucc]").
-  {
-    iFrame "#".
-    rewrite /zero_val /=. iFrame.
-  }
-  iIntros (e) "HshardCondPutPost".
-  wp_pures.
-  wp_if_destruct.
-  {
-    iRight.
-    iModIntro.
-    iSplitL ""; first done.
-    wp_pures.
-    iDestruct "HshardCondPutPost" as "(HshardCk & [[%Hbad _]|[_ Hpost]])".
-    { by exfalso. }
-    iDestruct "Hpost" as (succ) "(Hsucc & HΦ)".
-    wp_load.
-    iApply "HΦ". iModIntro.
-    iDestruct ("HcloseShardSet" with "HshardCk") as "HshardSet".
-    iDestruct ("HslClose" with "Hsmall_sl") as "?".
-    iFrame. iExists _, _, _, _. by iFrame "#∗".
-  }
-  {
-    wp_loadField.
-    iDestruct "HshardCondPutPost" as "(HshardCk & [Hatomic|[%Hbad _]])"; last first.
-    { exfalso. naive_solver. }
-    iDestruct ("HcloseShardSet" with "HshardCk") as "HshardSet".
-    wp_apply (wp_MemKVCoordClerk__GetShardMap with "[$HcoordCk_own]").
-    iIntros (shardMap_sl' shardMapping') "(HcoordCk_own & HshardMap_sl & %Hlength & #HshardServers')".
-    wp_apply (wp_storeField with "HshardMap").
-    { apply slice_val_ty. }
-    iIntros "HshardMap".
-    wp_pures.
-    iLeft.
-    iModIntro.
-
-    iSplitL ""; first done.
-    iDestruct "Hatomic" as "(_ & $ & Hsucc)".
-    iFrame.
-    iExists _,_,_,_; by iFrame "#∗".
-  }
+  {{{ RET #(bool_decide (expv = oldv)); True }}}.
+Proof.
+  iIntros "!#" (Φ) "#[Hp Hsl] Hatomic". wp_lam.
+  wp_apply (wp_KVClerk__getSeqClerk with "Hp").
+  iIntros (ck) "Hck".
+  wp_apply (wp_SeqKVClerk__ConditionalPut with "[$Hck $Hsl]").
+  iMod "Hatomic" as (oldv) "[Hkv HΦ]".
+  iModIntro. iExists oldv. iFrame "Hkv".
+  iIntros "Hkv". iMod ("HΦ" with "Hkv") as "HΦ".
+  iIntros "!> Hck".
+  wp_apply (wp_KVClerk__putSeqClerk with "Hp Hck").
+  wp_pures. iApply "HΦ". done.
 Qed.
 
-End memkv_clerk_proof.
+Lemma wp_KVClerk__MGet (p:loc) (γ:gname) (keys_sl:Slice.t) (keys_vals:list (u64 * list u8)) q :
+  {{{ is_KVClerk p γ ∗
+      is_slice_small keys_sl uint64T q (keys_vals.*1) ∗
+      [∗ list] key_val ∈ keys_vals, kvptsto γ key_val.1 key_val.2
+  }}}
+    KVClerk__MGet #p (slice_val keys_sl) @ ⊤
+  {{{ (vals_sl:Slice.t) (val_sls:list Slice.t), RET slice_val vals_sl;
+      is_slice_small keys_sl uint64T q (keys_vals.*1) ∗
+      is_slice_small vals_sl (slice.T byteT) 1 val_sls ∗
+      [∗ list] key_val;sl ∈ keys_vals;val_sls, kvptsto γ key_val.1 key_val.2 ∗
+        readonly (is_slice_small sl byteT 1 key_val.2)
+  }}}.
+Proof using Type*.
+  iIntros (Φ) "(#Hclerk & Hkeys_sl & Hkeys) HΦ". wp_lam.
+  wp_apply wp_slice_len.
+  wp_apply (wp_NewSlice (V:=Slice.t)).
+  iIntros (vals_sl) "Hvals_sl".
+  wp_apply wp_slice_len.
+
+  iDestruct (is_slice_small_sz with "Hkeys_sl") as %Hlen.
+  rewrite fmap_length in Hlen.
+  iDestruct (is_slice_to_small with "Hvals_sl") as "Hvals_sl".
+  iEval (rewrite /is_slice_small /slice.is_slice_small ?untype_replicate ?replicate_length)
+    in "Hkeys_sl Hvals_sl".
+  iDestruct "Hkeys_sl" as "[Hkeys_sl %Hkeys_sl_len]".
+  iDestruct "Hvals_sl" as "[Hvals_sl %Hvals_sl_len]".
+  wp_apply (wp_Multipar (X:=(u64 * list u8))
+    (λ i '(key, val),
+      (keys_sl.(Slice.ptr) +ₗ[uint64T] i) ↦[uint64T]{q} #key ∗
+      kvptsto γ key val ∗
+      (vals_sl.(Slice.ptr) +ₗ[slice.T byteT] i) ↦[slice.T byteT] slice_val Slice.nil)%I
+    (λ i kv, ∃ (val_sl:Slice.t), let '(key, val) := kv in
+      (keys_sl.(Slice.ptr) +ₗ[uint64T] i) ↦[uint64T]{q} #key ∗
+      kvptsto γ key val ∗
+      (vals_sl.(Slice.ptr) +ₗ[slice.T byteT] i) ↦[slice.T byteT] slice_val val_sl ∗
+      readonly (is_slice_small val_sl byteT 1 val))%I
+    keys_sl.(Slice.sz)
+    keys_vals
+    with "[] [Hkeys_sl Hkeys Hvals_sl]").
+  { done. }
+  {
+    iIntros "!> %i %kv %Hi Hpre". destruct kv as [key val].
+    iDestruct "Hpre" as "(Hkey_l & Hkey & Hval_l)".
+    wp_pures.
+
+    (* Breaking the SLiceGet (and later SliceSet) abstraction -- we only
+       own that one element, not the entire slice! *)
+    rewrite /SliceGet. wp_pures.
+    wp_apply wp_slice_ptr. wp_pures.
+    replace (int.nat i : Z) with (int.Z i) by word.
+    wp_load.
+
+    wp_apply (wp_KVClerk__Get_seq with "[$Hkey //]").
+    iIntros (val_sl qval_sl) "(Hkey & Hval_sl)".
+
+    rewrite /SliceSet. wp_pures.
+    wp_apply wp_slice_ptr. wp_pures.
+    wp_store.
+
+    iExists _.
+    iMod (readonly_alloc with "[Hval_sl]") as "$"; first done.
+    eauto with iFrame. }
+  { rewrite /array /list.untype !big_sepL_fmap.
+    iDestruct (big_sepL2_sepL_2 with "Hkeys_sl Hvals_sl") as "Hsl".
+    { rewrite Hlen replicate_length //. }
+    rewrite big_sepL2_replicate_r //.
+    iCombine "Hkeys Hsl" as "H". rewrite -big_sepL_sep.
+    iApply (big_sepL_impl with "H").
+    iIntros "!> %i %kv %Hi (Hkey & Hkey_sl & Hval_sl)".
+    destruct kv as [key value].
+    iFrame. }
+  iIntros "H".
+  wp_pures.
+  iDestruct (big_sepL_exists_to_sepL2 with "H") as (xs) "H".
+  iDestruct (big_sepL2_length with "H") as %Hlenxs.
+  iApply ("HΦ" $! vals_sl xs). iModIntro.
+  iEval (rewrite {1 2}/is_slice_small /slice.is_slice_small).
+  rewrite /array /list.untype !big_sepL_fmap !fmap_length.
+  iEval (rewrite [(_ ∗ ⌜length keys_vals = _⌝)%I]comm -!assoc).
+  iSplit; first done.
+  iEval (rewrite !assoc [(_ ∗ ⌜length xs = _⌝)%I]comm -!assoc).
+  rewrite -Hlenxs Hlen. iSplit; first done.
+  iEval (rewrite [(([∗ list] k↦y ∈ xs, _) ∗ _)%I]comm).
+  rewrite -big_sepL2_sep_sepL_r.
+  rewrite -big_sepL2_sep_sepL_l.
+  iApply (big_sepL2_impl with "H").
+  iIntros "!> %i %kv %val_sl %Hi1 %Hi2". destruct kv as [key val].
+  iIntros "(Hkeys_sl & Hkey & Hvals_sl & Hval_sl)". iFrame.
+Qed.
+
+End memkv_concurrent_clerk_proof.
