src/program_proof/memkv/memkv_get_proof.v
@@ -39,7 +39,7 @@ Qed.
 Local Ltac Zify.zify_post_hook ::= Z.div_mod_to_equations.
 
 Lemma wp_GetRPC (s args_ptr reply_ptr:loc) args γ γreq Q :
-  is_MemKVShardServer s γ -∗
+  is_KVShardServer s γ -∗
   {{{
        own_GetRequest args_ptr args ∗
        (∃ dummy_rep, own_GetReply reply_ptr dummy_rep) ∗
@@ -47,7 +47,7 @@ Lemma wp_GetRPC (s args_ptr reply_ptr:loc) args γ γreq Q :
                                 (PostShardGet γ.(kv_gn) args.(GR_Key) Q)
                                 {| Req_CID:=args.(GR_CID); Req_Seq:=args.(GR_Seq) |}
   }}}
-    MemKVShardServer__GetRPC #s #args_ptr #reply_ptr
+    KVShardServer__GetRPC #s #args_ptr #reply_ptr
   {{{
        rep, RET #();
        own_GetReply reply_ptr rep ∗
