src/program_proof/memkv/memkv_seq_clerk_proof.v
@@ -1,0 +1,383 @@
+From Perennial.program_proof Require Import grove_prelude std_proof.
+From Goose.github_com.mit_pdos.gokv Require Import memkv.
+From Perennial.program_proof.lockservice Require Import rpc.
+From Perennial.program_logic Require Import atomic_fupd.
+From Perennial.program_proof.memkv Require Export common_proof memkv_coord_definitions memkv_coord_clerk_proof memkv_shard_clerk_proof.
+
+Section memkv_clerk_proof.
+
+Context `{!heapGS Σ (ext:=grove_op) (ffi:=grove_model), !rpcG Σ ShardReplyC, !rpcregG Σ, !kvMapG Σ}.
+
+Definition own_SeqKVClerk (ck:loc) (γ:gname) : iProp Σ :=
+  ∃ (s coordCk:loc) shardMap_sl (shardMapping:list u64),
+  "HshardClerks" ∷ ck ↦[SeqKVClerk :: "shardClerks"] #s ∗
+  "HshardClerksSet" ∷ own_ShardClerkSet s γ ∗
+  "HcoordCk" ∷ ck ↦[SeqKVClerk :: "coordCk"] #coordCk ∗
+  "HcoordCk_own" ∷ own_KVCoordClerk coordCk γ ∗
+  "HshardMap" ∷ ck ↦[SeqKVClerk :: "shardMap"] (slice_val shardMap_sl) ∗
+  "HshardMap_sl" ∷ is_slice shardMap_sl uint64T 1%Qp shardMapping ∗
+  "%HshardMap_length" ∷ ⌜Z.of_nat (length shardMapping) = uNSHARD⌝ ∗
+  "#HshardServers" ∷ all_are_shard_servers shardMapping γ
+.
+
+Lemma wp_MakeSeqKVClerk (coord:u64) cm γ :
+  {{{
+       is_coord_server coord γ ∗ is_ConnMan cm
+  }}}
+    MakeSeqKVClerk #coord #cm
+  {{{
+       (ck:loc), RET #ck; own_SeqKVClerk ck γ.(coord_kv_gn)
+  }}}
+.
+Proof.
+  iIntros (Φ) "[#Hcoord #Hcm] HΦ".
+  wp_lam.
+  wp_apply (wp_allocStruct).
+  { Transparent slice.T. repeat econstructor.  Opaque slice.T. }
+  iIntros (cck) "Hcck".
+  wp_pures.
+  wp_apply (wp_allocStruct).
+  { Transparent slice.T. repeat econstructor.  Opaque slice.T. }
+  iIntros (ck) "Hck".
+  iDestruct (struct_fields_split with "Hck") as "HH".
+  iNamed "HH".
+  iDestruct (struct_fields_split with "Hcck") as "HH".
+  iNamed "HH".
+  wp_pures.
+  wp_storeField.
+  wp_loadField.
+  wp_storeField.
+  wp_loadField.
+  wp_storeField.
+  wp_bind (MakeShardClerkSet _).
+  wp_lam.
+  replace (ref (InjLV #null))%E with (NewMap (struct.ptrT KVShardClerk)) by auto.
+  wp_apply (wp_NewMap).
+  iIntros (mref_set) "Hmap_set".
+  wp_apply (wp_allocStruct).
+  { eauto. }
+  iIntros (clset) "Hset".
+  wp_storeField.
+  wp_loadField.
+  wp_apply (wp_KVCoordClerk__GetShardMap with "[c host]").
+  { rewrite /own_KVCoordClerk. iExists _, _, _. iFrame "c host Hcm".
+    iSplit; last first.
+    { iExact "Hcoord". }
+    done.
+  }
+  iIntros (shardMap_sl shardMapping) "(Hcck & HshardMap_sl & %Hlen & #Hall_are_shard_servers)".
+  Transparent slice.T.
+  wp_storeField.
+  Opaque slice.T.
+  iModIntro. iApply "HΦ".
+  iExists _, _, _, _. iFrame.
+  iFrame "% #". iExists _, _, _.
+  iFrame "Hmap_set Hcm".
+  iDestruct (struct_fields_split with "Hset") as "HH".
+  iNamed "HH". iFrame.
+  rewrite big_sepM_empty; done.
+Qed.
+
+Lemma wp_SeqKVClerk__Get (ck:loc) (γ:gname) (key:u64) :
+⊢ {{{ own_SeqKVClerk ck γ }}}
+  <<< ∀∀ v, kvptsto γ key v >>>
+    SeqKVClerk__Get #ck #key @ ∅
+  <<< kvptsto γ key v >>>
+  {{{ val_sl q, RET slice_val val_sl;
+      own_SeqKVClerk ck γ ∗ is_slice_small val_sl byteT q%Qp v
+  }}}.
+Proof using Type*.
+  iIntros "!#" (Φ) "Hown Hatomic".
+  wp_lam.
+  wp_pures.
+  wp_apply wp_ref_of_zero.
+  { done. }
+  iIntros (rep_ptr) "Hrep".
+  wp_pures.
+
+  (* Weaken assumption for loop invariant *)
+  iAssert (∃ rep_sl, rep_ptr ↦[slice.T byteT] (slice_val rep_sl) )%I with "[Hrep]" as "Hrep".
+  {
+    rewrite zero_slice_val.
+    iExists _; iFrame.
+  }
+
+  wp_forBreak.
+  wp_pures.
+
+  wp_apply (wp_shardOf_bound).
+  iIntros (sid HsidLe).
+  wp_pures.
+
+  iNamed "Hown".
+  wp_loadField.
+  iDestruct (is_slice_small_acc with "HshardMap_sl") as "[Hsmall_sl HslClose]".
+
+  assert (int.nat sid < length shardMapping)%nat as HsidLe_nat by word.
+  eapply list_lookup_lt in HsidLe_nat.
+  destruct HsidLe_nat as [hostID HsidLe_nat].
+  wp_apply (wp_SliceGet (V:=u64) with "[$Hsmall_sl]").
+  {
+    iPureIntro.
+    done.
+  }
+  iIntros "Hsmall_sl".
+  wp_pures.
+  wp_loadField.
+
+  unfold all_are_shard_servers.
+  iDestruct ("HshardServers" $! (int.nat sid) hostID HsidLe_nat) as "HH".
+  iNamed "HH".
+
+  wp_apply (wp_ShardClerkSet__GetClerk with "[$HshardClerksSet]").
+  { iFrame "HH". }
+  iClear "HH".
+
+  iIntros (?) "(HshardCk & HcloseShardSet)".
+
+  wp_pures.
+  rewrite difference_empty_L.
+  wp_apply (wp_KVShardClerk__Get with "[Hatomic $HshardCk $Hrep]").
+  {
+    iFrame "Hatomic".
+  }
+  iIntros (e) "HshardGetPost".
+  wp_pures.
+  wp_if_destruct.
+  {
+    iRight.
+    iModIntro.
+    iSplitL ""; first done.
+    wp_pures.
+    iDestruct "HshardGetPost" as "(HshardCk & [[%Hbad _]|[_ Hpost]])".
+    { by exfalso. }
+    iNamed "Hpost".
+    iDestruct "Hpost" as "(Hrep & Hval_sl & HΦ)".
+    wp_load.
+    iMod (readonly_load with "Hval_sl") as (?) "Hval_sl".
+    iModIntro.
+    iApply "HΦ".
+    iFrame.
+    iDestruct ("HcloseShardSet" with "HshardCk") as "HshardSet".
+    iDestruct ("HslClose" with "Hsmall_sl") as "?".
+    iExists _, _, _, _. by iFrame "#∗".
+  }
+  {
+    wp_loadField.
+    iDestruct "HshardGetPost" as "(HshardCk & [Hatomic|[%Hbad _]])"; last first.
+    { exfalso. naive_solver. }
+    iDestruct ("HcloseShardSet" with "HshardCk") as "HshardSet".
+    wp_apply (wp_KVCoordClerk__GetShardMap with "[$HcoordCk_own]").
+    iIntros (shardMap_sl' shardMapping') "(HcoordCk_own & HshardMap_sl & %Hlength & #HshardServers')".
+    wp_apply (wp_storeField with "HshardMap").
+    { apply slice_val_ty. }
+    iIntros "HshardMap".
+    wp_pures.
+    iLeft.
+    iModIntro.
+
+    iSplitL ""; first done.
+    iDestruct "Hatomic" as "[_ $]".
+    iExists _,_,_,_; by iFrame "#∗".
+  }
+Qed.
+
+(* Sequential spec *)
+Lemma wp_SeqKVClerk__Get_seq (ck:loc) (γ:gname) (key:u64) (v:list u8) :
+  {{{ own_SeqKVClerk ck γ ∗ kvptsto γ key v }}}
+    SeqKVClerk__Get #ck #key @ ⊤
+  {{{ val_sl q, RET slice_val val_sl;
+      own_SeqKVClerk ck γ ∗ kvptsto γ key v ∗ is_slice_small val_sl byteT q%Qp v
+  }}}.
+Proof using Type*.
+  iIntros (Φ) "(Hclerk & Hkey) HΦ".
+  iApply (wp_SeqKVClerk__Get with "Hclerk").
+  iApply fupd_mask_intro; first done. iNext.
+  iIntros "Hclose". iExists _. iFrame "Hkey".
+  iIntros "Hkey". iMod "Hclose" as "_". iModIntro.
+  iIntros (??) "[Hclerk Hsl]". iApply "HΦ". iFrame.
+Qed.
+
+Lemma wp_SeqKVClerk__Put (ck:loc) (γ:gname) (key:u64) (val_sl:Slice.t) (v:list u8):
+⊢ {{{ own_SeqKVClerk ck γ ∗ readonly (is_slice_small val_sl byteT 1 v) }}}
+  <<< ∀∀ oldv, kvptsto γ key oldv >>>
+    SeqKVClerk__Put #ck #key (slice_val val_sl) @ ∅
+  <<< kvptsto γ key v >>>
+  {{{ RET #(); own_SeqKVClerk ck γ }}}.
+Proof using Type*.
+  iIntros "!#" (Φ) "[Hown #Hval_sl] Hatomic".
+  wp_lam.
+  wp_pures.
+
+  wp_forBreak.
+  wp_pures.
+
+  wp_apply (wp_shardOf_bound).
+  iIntros (sid HsidLe).
+  wp_pures.
+
+  iNamed "Hown".
+  wp_loadField.
+  iDestruct (is_slice_small_acc with "HshardMap_sl") as "[Hsmall_sl HslClose]".
+
+  assert (int.nat sid < length shardMapping)%nat as HsidLe_nat by word.
+  eapply list_lookup_lt in HsidLe_nat.
+  destruct HsidLe_nat as [hostID HsidLe_nat].
+  wp_apply (wp_SliceGet (V:=u64) with "[$Hsmall_sl]").
+  {
+    iPureIntro.
+    done.
+  }
+  iIntros "Hsmall_sl".
+  wp_pures.
+  wp_loadField.
+
+  unfold all_are_shard_servers.
+  iDestruct ("HshardServers" $! (int.nat sid) hostID HsidLe_nat) as "HH".
+  iNamed "HH".
+  wp_apply (wp_ShardClerkSet__GetClerk with "[$HshardClerksSet $HH]").
+  iClear "HH".
+
+  iIntros (?) "(HshardCk & HcloseShardSet)".
+
+  wp_pures.
+  rewrite difference_empty_L.
+  wp_apply (wp_KVShardClerk__Put with "[Hatomic $Hval_sl $HshardCk]").
+  {
+    iFrame "Hatomic".
+  }
+  iIntros (e) "HshardPutPost".
+  wp_pures.
+  wp_if_destruct.
+  {
+    iRight.
+    iModIntro.
+    iSplitL ""; first done.
+    wp_pures.
+    iDestruct "HshardPutPost" as "(HshardCk & [[%Hbad _]|[_ Hpost]])".
+    { by exfalso. }
+    iApply "Hpost".
+    iDestruct ("HcloseShardSet" with "HshardCk") as "HshardSet".
+    iDestruct ("HslClose" with "Hsmall_sl") as "?".
+    iModIntro. iExists _, _, _, _. by iFrame "#∗".
+  }
+  {
+    wp_loadField.
+    iDestruct "HshardPutPost" as "(HshardCk & [Hatomic|[%Hbad _]])"; last first.
+    { exfalso. naive_solver. }
+    iDestruct ("HcloseShardSet" with "HshardCk") as "HshardSet".
+    wp_apply (wp_KVCoordClerk__GetShardMap with "[$HcoordCk_own]").
+    iIntros (shardMap_sl' shardMapping') "(HcoordCk_own & HshardMap_sl & %Hlength & #HshardServers')".
+    wp_apply (wp_storeField with "HshardMap").
+    { apply slice_val_ty. }
+    iIntros "HshardMap".
+    wp_pures.
+    iLeft.
+    iModIntro.
+
+    iSplitL ""; first done.
+    iDestruct "Hatomic" as "[_ $]".
+    iFrame.
+    iExists _,_,_,_. by iFrame "#∗".
+  }
+Qed.
+
+Lemma wp_SeqKVClerk__ConditionalPut (ck:loc) (γ:gname) (key:u64) (expv_sl newv_sl:Slice.t) (expv newv:list u8):
+⊢ {{{ own_SeqKVClerk ck γ ∗
+      readonly (is_slice_small expv_sl byteT 1 expv) ∗
+      readonly (is_slice_small newv_sl byteT 1 newv) }}}
+  <<< ∀∀ oldv, kvptsto γ key oldv >>>
+    SeqKVClerk__ConditionalPut #ck #key (slice_val expv_sl) (slice_val newv_sl) @ ∅
+  <<< kvptsto γ key (if bool_decide (expv = oldv) then newv else oldv) >>>
+  {{{ RET #(bool_decide (expv = oldv));
+      own_SeqKVClerk ck γ }}}.
+Proof using Type*.
+  iIntros "!#" (Φ) "(Hown & #Hexpv_sl & #Hnewv_sl) Hatomic".
+  wp_lam.
+  wp_pures.
+  wp_apply (wp_ref_of_zero _ _ boolT).
+  { done. }
+  iIntros (succ_ptr) "Hsucc".
+  wp_pures.
+  (* Weaken assumption for loop invariant *)
+  iAssert (∃ b:bool, succ_ptr ↦[boolT] #b)%I with "[Hsucc]" as "Hsucc".
+  { iExists _. done. }
+
+  wp_forBreak.
+  wp_pures.
+
+  wp_apply (wp_shardOf_bound).
+  iIntros (sid HsidLe).
+  wp_pures.
+
+  iNamed "Hown".
+  wp_loadField.
+  iDestruct (is_slice_small_acc with "HshardMap_sl") as "[Hsmall_sl HslClose]".
+
+  assert (int.nat sid < length shardMapping)%nat as HsidLe_nat by word.
+  eapply list_lookup_lt in HsidLe_nat.
+  destruct HsidLe_nat as [hostID HsidLe_nat].
+  wp_apply (wp_SliceGet (V:=u64) with "[$Hsmall_sl]").
+  {
+    iPureIntro.
+    done.
+  }
+  iIntros "Hsmall_sl".
+  wp_pures.
+  wp_loadField.
+
+  unfold all_are_shard_servers.
+  iDestruct ("HshardServers" $! (int.nat sid) hostID HsidLe_nat) as "HH".
+  iNamed "HH".
+  wp_apply (wp_ShardClerkSet__GetClerk with "[$HshardClerksSet $HH]").
+  iClear "HH".
+
+  iIntros (?) "(HshardCk & HcloseShardSet)".
+
+  wp_pures.
+  rewrite difference_empty_L.
+  wp_apply (wp_KVShardClerk__ConditionalPut _ _ _ _ _ _ _ _ (λ b, own_SeqKVClerk ck γ -∗ Φ #b)%I
+    with "[Hatomic $HshardCk Hsucc]").
+  {
+    iFrame "#".
+    rewrite /zero_val /=. iFrame.
+  }
+  iIntros (e) "HshardCondPutPost".
+  wp_pures.
+  wp_if_destruct.
+  {
+    iRight.
+    iModIntro.
+    iSplitL ""; first done.
+    wp_pures.
+    iDestruct "HshardCondPutPost" as "(HshardCk & [[%Hbad _]|[_ Hpost]])".
+    { by exfalso. }
+    iDestruct "Hpost" as (succ) "(Hsucc & HΦ)".
+    wp_load.
+    iApply "HΦ". iModIntro.
+    iDestruct ("HcloseShardSet" with "HshardCk") as "HshardSet".
+    iDestruct ("HslClose" with "Hsmall_sl") as "?".
+    iFrame. iExists _, _, _, _. by iFrame "#∗".
+  }
+  {
+    wp_loadField.
+    iDestruct "HshardCondPutPost" as "(HshardCk & [Hatomic|[%Hbad _]])"; last first.
+    { exfalso. naive_solver. }
+    iDestruct ("HcloseShardSet" with "HshardCk") as "HshardSet".
+    wp_apply (wp_KVCoordClerk__GetShardMap with "[$HcoordCk_own]").
+    iIntros (shardMap_sl' shardMapping') "(HcoordCk_own & HshardMap_sl & %Hlength & #HshardServers')".
+    wp_apply (wp_storeField with "HshardMap").
+    { apply slice_val_ty. }
+    iIntros "HshardMap".
+    wp_pures.
+    iLeft.
+    iModIntro.
+
+    iSplitL ""; first done.
+    iDestruct "Hatomic" as "(_ & $ & Hsucc)".
+    iFrame.
+    iExists _,_,_,_; by iFrame "#∗".
+  }
+Qed.
+
+End memkv_clerk_proof.
